@prefix era-sh: <http://data.europa.eu/949/shapes/> .
@prefix ex: <http://example.org/ns#> .
@prefix sh: <http://www.w3.org/ns/shacl#> .
@prefix xsd: <http://www.w3.org/2001/XMLSchema#> .
@prefix rdf: <http://www.w3.org/1999/02/22-rdf-syntax-ns#> .
@prefix rdfs: <http://www.w3.org/2000/01/rdf-schema#> .
@prefix era: <http://data.europa.eu/949/> .
@prefix era-sn: <http://data.europa.eu/949/concepts/sol-natures/> .
@prefix skos: <http://www.w3.org/2004/02/skos/core#> .
@prefix wgs: <http://www.w3.org/2003/01/geo/wgs84_pos#> .
@prefix geosparql: <http://www.opengis.net/ont/geosparql#> .
@prefix era-ph: <http://data.europa.eu/949/concepts/platform-heights/> .
@prefix era-tenclass: <http://data.europa.eu/949/concepts/ten-classifications/> .
@prefix era-gaugings: <http://data.europa.eu/949/concepts/gaugings/> .
@prefix era-ntg: <http://data.europa.eu/949/concepts/nominal-track-gauges/> .
@prefix era-tds: <http://data.europa.eu/949/concepts/train-detection/> .
@prefix era-tdssc: <http://data.europa.eu/949/concepts/train-detection-specific-checks/> .
@prefix era-tsi: <http://data.europa.eu/949/concepts/tsi-compliances/> .
@prefix era-malvc: <http://data.europa.eu/949/concepts/min-axle-loads-per-vehicle-category/> .
@prefix era-mas: <http://data.europa.eu/949/concepts/max-amount-sandings/> .

#############################
# Rules for train detection system
#############################

era-sh:TrainDetectionSystemShape
	a sh:NodeShape ;
	sh:targetClass era:TrainDetectionSystem .    # Applies to all TrainDetectionSystem instances

# train-detection-system : # 1.1.1.3.7.1.1
era-sh:TrainDetectionSystemShape sh:property era-sh:trainDetectionSystem .
era-sh:trainDetectionSystem
	a sh:PropertyShape ;
	rdfs:comment "Indication of types of train detection system installed." ;
	era:rinfIndex "1.1.1.3.7.1.1" ;
	sh:path era:trainDetectionSystem ;
	sh:minCount 0 ; # TODO: Not yet applicable
	sh:nodeKind sh:IRI ;
#	sh:class skos:Concept ; #TODO: Check error
	sh:inScheme era-tds:TrainDetectionSystems ;
	sh:severity sh:Violation ;
	sh:message "trainDetectionSystem (1.1.1.3.7.1.1): Indication of types of train detection system installed."@en .

# trainDetectionSystemSpecificCheck: # 1.1.1.3.7.1.2
era-sh:TrainDetectionSystemShape sh:property era-sh:trainDetectionSystemSpecificCheck .
era-sh:trainDetectionSystemSpecificCheck
	a sh:PropertyShape ;
	rdfs:comment "Indication of types of train detection system to which specific checks are needed." ;
	era:rinfIndex "1.1.1.3.7.1.2" ;
	sh:path era:trainDetectionSystemSpecificCheck ;
	sh:minCount 0 ; # TODO: Not yet applicable
	sh:nodeKind sh:IRI ;
#	sh:class skos:Concept ; #TODO: Check error
	sh:inScheme era-tdssc:TrainDetectionSystemsSpecificChecks ;
	sh:severity sh:Violation ;
	sh:message "trainDetectionSystemSpecificCheck (1.1.1.3.7.1.2): Indication of types of train detection system to which specific checks are needed."@en .

# tsiCompliantMaxDistConsecutiveAxles: # 1.1.1.3.7.2.1
era-sh:TrainDetectionSystemShape sh:property era-sh:tsiCompliantMaxDistConsecutiveAxles .
era-sh:tsiCompliantMaxDistConsecutiveAxles
	a sh:PropertyShape ;
	rdfs:comment "Indication whether the maximum distance between consecutive axles is TSI compliant." ;
	era:rinfIndex "1.1.1.3.7.2.1" ;
	sh:path era:tsiCompliantMaxDistConsecutiveAxles ;
	sh:minCount 0 ; # TODO: Not yet applicable
	sh:nodeKind sh:IRI ;
#	sh:class skos:Concept ; #TODO: Check error
	sh:inScheme era-tsi:TSICompliances ;
	sh:severity sh:Violation ;
	sh:message "tsiCompliantMaxDistConsecutiveAxles (1.1.1.3.7.2.1): Indication whether the maximum distance between consecutive axles is TSI compliant."@en .

# maxDistConsecutiveAxles: # 1.1.1.3.7.2.2
era-sh:TrainDetectionSystemShape sh:property era-sh:maxDistConsecutiveAxles .
era-sh:maxDistConsecutiveAxles
	a sh:PropertyShape ;
	rdfs:comment "Indication of maximum permitted distance between two consecutive axles in case of TSI non-compliance, given millimetres." ;
	era:rinfIndex "1.1.1.3.7.2.2" ;
	sh:path era:maxDistConsecutiveAxles ;
	sh:minCount 0 ; # TODO: Not yet applicable
	sh:datatype xsd:integer ;
	sh:pattern "^([1-9]\\d{1,4}|[0-9])$" ;
	sh:severity sh:Violation ;
	sh:message "maxDistConsecutiveAxles (1.1.1.3.7.2.2): Indication of maximum permitted distance between two consecutive axles in case of TSI non-compliance, given millimetres."@en .

# minDistConsecutiveAxles: # 1.1.1.3.7.3
era-sh:TrainDetectionSystemShape sh:property era-sh:minDistConsecutiveAxles .
era-sh:minDistConsecutiveAxles
	a sh:PropertyShape ;
	rdfs:comment "Indication of minimum permitted distance between two consecutive axles, given millimetres." ;
	era:rinfIndex "1.1.1.3.7.3" ;
	sh:path era:minDistConsecutiveAxles ;
	sh:minCount 0 ; # TODO: Not yet applicable
	sh:datatype xsd:integer ;
	sh:pattern "^([1-9]\\d{1,3}|[0-9])$" ;
	sh:severity sh:Violation ;
	sh:message "minDistConsecutiveAxles (1.1.1.3.7.3): Indication of minimum permitted distance between two consecutive axles, given millimetres."@en .

# minDistFirstLastAxle: # 1.1.1.3.7.4
era-sh:TrainDetectionSystemShape sh:property era-sh:minDistFirstLastAxle .
era-sh:minDistFirstLastAxle
	a sh:PropertyShape ;
	rdfs:comment "Indication of minimum permitted distance between the first and last axles, given millimetres." ;
	era:rinfIndex "1.1.1.3.7.4" ;
	sh:path era:minDistFirstLastAxle ;
	sh:minCount 0 ; # TODO: Not yet applicable
	sh:datatype xsd:integer ;
	sh:pattern "^([1-9]\\d{1,4}|[0-9])$" ;
	sh:severity sh:Violation ;
	sh:message "minDistFirstLastAxle (1.1.1.3.7.4): Indication of minimum permitted distance between the first and last axles, given millimetres."@en .

# maxDistEndTrainFirstAxle: # 1.1.1.3.7.5
era-sh:TrainDetectionSystemShape sh:property era-sh:maxDistEndTrainFirstAxle .
era-sh:maxDistEndTrainFirstAxle
	a sh:PropertyShape ;
	rdfs:comment "Indication of maximum permitted distance between the end of the train and the first axle, given millimetres." ;
	era:rinfIndex "1.1.1.3.7.5" ;
	sh:path era:maxDistEndTrainFirstAxle ;
	sh:minCount 0 ; # TODO: Not yet applicable
	sh:datatype xsd:integer ;
	sh:pattern "^([1-9]\\d{1,3}|[0-9])$" ;
	sh:severity sh:Violation ;
	sh:message "maxDistEndTrainFirstAxle (1.1.1.3.7.5): Indication of maximum permitted distance between the end of the train and the first axle, given millimetres."@en .

# minRimWidth: # 1.1.1.3.7.6
era-sh:TrainDetectionSystemShape sh:property era-sh:minRimWidth .
era-sh:minRimWidth
	a sh:PropertyShape ;
	rdfs:comment "Indication of minimum permitted rim width, given millimetres." ;
	era:rinfIndex "1.1.1.3.7.6" ;
	sh:path era:minRimWidth ;
	sh:minCount 0 ; # TODO: Not yet applicable
	sh:datatype xsd:double ;
	sh:pattern "^([1-9]\\d{1,2}|[0-9])$" ;
	sh:severity sh:Violation ;
	sh:message "minRimWidth (1.1.1.3.7.6): Indication of minimum permitted rim width, given millimetres."@en .
	
# minWheelDiameter: # 1.1.1.3.7.7
era-sh:TrainDetectionSystemShape sh:property era-sh:minWheelDiameter .
era-sh:minWheelDiameter
	a sh:PropertyShape ;
	rdfs:comment "Indication of minimum permitted wheel diameter, given millimetres." ;
	era:rinfIndex "1.1.1.3.7.7" ;
	sh:path era:minWheelDiameter ;
	sh:minCount 0 ; # TODO: Not yet applicable
	sh:datatype xsd:integer ;
	sh:pattern "^([1-9]\\d{1,2}|[0-9])$" ;
	sh:severity sh:Violation ;
	sh:message "minWheelDiameter (1.1.1.3.7.7): Indication of minimum permitted wheel diameter, given millimetres."@en .

# minFlangeThickness: # 1.1.1.3.7.8
era-sh:TrainDetectionSystemShape sh:property era-sh:minFlangeThickness .
era-sh:minFlangeThickness
	a sh:PropertyShape ;
	rdfs:comment "Indication of minimum permitted flange thickness, given millimetres." ;
	era:rinfIndex "1.1.1.3.7.8" ;
	sh:path era:minFlangeThickness ;
	sh:minCount 0 ; # TODO: Not yet applicable
	sh:datatype xsd:double ;
	sh:pattern "^([1-9]{0,1}[0-9]\\.[0-9])$" ;
	sh:severity sh:Violation ;
	sh:message "minFlangeThickness (1.1.1.3.7.8): Indication of minimum permitted flange thickness, given millimetres."@en .

# minFlangeHeight: # 1.1.1.3.7.9
era-sh:TrainDetectionSystemShape sh:property era-sh:minFlangeHeight .
era-sh:minFlangeHeight
	a sh:PropertyShape ;
	rdfs:comment "Indication of minimum permitted flange height, given millimetres." ;
	era:rinfIndex "1.1.1.7.9" ;
	sh:path era:minFlangeHeight ;
	sh:minCount 0 ; # TODO: Not yet applicable
	sh:datatype xsd:double ;
	sh:pattern "^([1-9]{0,1}[0-9]\\.[0-9])$" ;
	sh:severity sh:Violation ;
	sh:message "minFlangeHeight (1.1.1.7.9): Indication of minimum permitted flange height, given millimetres."@en .

# maxFlangeHeight: # 1.1.1.3.7.10
era-sh:TrainDetectionSystemShape sh:property era-sh:maxFlangeHeight .
era-sh:maxFlangeHeight
	a sh:PropertyShape ;
	rdfs:comment "Indication of maximum permitted flange height, given millimetres." ;
	era:rinfIndex "1.1.1.3.7.10" ;
	sh:path era:maxFlangeHeight ;
	sh:minCount 0 ; # TODO: Not yet applicable
	sh:datatype xsd:double ;
	sh:pattern "^([1-9]{0,1}[0-9]\\.[0-9])$" ;
	sh:severity sh:Violation ;
	sh:message "maxFlangeHeight (1.1.1.3.7.10): Indication of maximum permitted flange height, given millimetres."@en .

# minAxleLoad: # 1.1.1.3.7.11
era-sh:TrainDetectionSystemShape sh:property era-sh:minAxleLoad .
era-sh:minAxleLoad
	a sh:PropertyShape ;
	rdfs:comment "Indication of minimum permitted axle load, given tonnes." ;
	era:rinfIndex "1.1.1.3.7.11" ;
	sh:path era:minAxleLoad ;
	sh:minCount 0 ; # TODO: Not yet applicable
	sh:datatype xsd:double ;
	sh:pattern "^([1-9]{0,1}[0-9]\\.[0-9])$" ;
	sh:severity sh:Violation ;
	sh:message "minAxleLoad (1.1.1.3.7.11): Indication of minimum permitted axle load, given tonnes."@en .

# minAxleLoadVehicleCategory: # 1.1.1.3.7.11.1
era-sh:TrainDetectionSystemShape sh:property era-sh:minAxleLoadVehicleCategory .
era-sh:minAxleLoadVehicleCategory
	a sh:PropertyShape ;
	rdfs:comment "Indication of minimum permitted axle load, given vehicle category." ;
	era:rinfIndex "1.1.1.3.7.11.1" ;
	sh:path era:minAxleLoadVehicleCategory ;
	sh:minCount 0 ; # TODO: Not yet applicable
	sh:nodeKind sh:IRI ;
#	sh:class skos:Concept ; #TODO: Check error
	skos:inScheme era-malvc:MinAxleLoadsPerVehicleCategory ;
	sh:severity sh:Violation ;
	sh:message "minAxleLoadVehicleCategory (1.1.1.3.7.11.1): Indication of minimum permitted axle load, given vehicle category."@en .

# tsiCompliantMetalFreeSpace: # 1.1.1.3.7.12
era-sh:TrainDetectionSystemShape sh:property era-sh:tsiCompliantMetalFreeSpace .
era-sh:tsiCompliantMetalFreeSpace
	a sh:PropertyShape ;
	rdfs:comment "Indication of whether the rules are TSI compliant for metal free space around wheels." ;
	era:rinfIndex "1.1.1.3.7.12" ;
	sh:path era:tsiCompliantMetalFreeSpace ;
	sh:minCount 0 ; # TODO: Not yet applicable
	sh:nodeKind sh:IRI ;
#	sh:class skos:Concept ; #TODO: Check error
	skos:inScheme era-tsi:TSICompliances ;
	sh:severity sh:Violation ;
	sh:message "tsiCompliantMetalFreeSpace (1.1.1.3.7.12): Indication of whether the rules are TSI compliant for metal free space around wheels."@en .

# tsiCompliantMetalConstruction: # 1.1.1.3.7.13
era-sh:TrainDetectionSystemShape sh:property era-sh:tsiCompliantMetalConstruction .
era-sh:tsiCompliantMetalConstruction
	a sh:PropertyShape ;
	rdfs:comment "Indication of whether the rules are TSI compliant for vehicle metal construction." ;
	era:rinfIndex "1.1.1.3.7.13" ;
	sh:path era:tsiCompliantMetalConstruction ;
	sh:minCount 0 ; # TODO: Not yet applicable
	sh:nodeKind sh:IRI ;
#	sh:class skos:Concept ; #TODO: Check error
	skos:inScheme era-tsi:TSICompliances ;
	sh:severity sh:Violation ;
	sh:message "tsiCompliantMetalConstruction (1.1.1.3.7.13): Indication of whether the rules are TSI compliant for vehicle metal construction."@en .

# tsiCompliantFerromagneticWheel: # 1.1.1.3.7.14
era-sh:TrainDetectionSystemShape sh:property era-sh:tsiCompliantFerromagneticWheel .
era-sh:tsiCompliantFerromagneticWheel
	a sh:PropertyShape ;
	rdfs:comment "Indication of whether the rules are TSI compliant for ferromagnetic characteristics of wheel material required." ;
	era:rinfIndex "1.1.1.3.7.14" ;
	sh:path era:tsiCompliantFerromagneticWheel ;
	sh:minCount 0 ; # TODO: Not yet applicable
	sh:nodeKind sh:IRI ;
#	sh:class skos:Concept ; #TODO: Check error
	skos:inScheme era-tsi:TSICompliances ;
	sh:severity sh:Violation ;
	sh:message "tsiCompliantFerromagneticWheel (1.1.1.3.7.14): Indication of whether the rules are TSI compliant for ferromagnetic characteristics of wheel material required."@en .

# tsiCompliantMaxImpedanceWheelset: # 1.1.1.3.7.15.1
era-sh:TrainDetectionSystemShape sh:property era-sh:tsiCompliantMaxImpedanceWheelset .
era-sh:tsiCompliantMaxImpedanceWheelset
	a sh:PropertyShape ;
	rdfs:comment "Indication of whether the rules are TSI compliant for maximum impedance between opposite wheels of a wheelset." ;
	era:rinfIndex "1.1.1.3.7.15.1" ;
	sh:path era:tsiCompliantMaxImpedanceWheelset ;
	sh:minCount 0 ; # TODO: Not yet applicable
	sh:nodeKind sh:IRI ;
#	sh:class skos:Concept ; #TODO: Check error
	skos:inScheme era-tsi:TSICompliances ;
	sh:severity sh:Violation ;
	sh:message "tsiCompliantMaxImpedanceWheelset (1.1.1.3.7.15.1): Indication of whether the rules are TSI compliant for maximum impedance between opposite wheels of a wheelset."@en .

# maxImpedanceWheelset: # 1.1.1.3.7.15.2
era-sh:TrainDetectionSystemShape sh:property era-sh:maxImpedanceWheelset .
era-sh:maxImpedanceWheelset
	a sh:PropertyShape ;
	rdfs:comment "Maximum impedance between opposite wheels of a wheelset when not TSI compilant." ;
	era:rinfIndex "1.1.1.3.7.15.2" ;
	sh:path era:maxImpedanceWheelset ;
	sh:minCount 0 ; # TODO: Not yet applicable
	sh:datatype xsd:double ;
	sh:pattern "^[0-9](\\.[0-9]{1,3})?$" ;
	sh:severity sh:Violation ;
	sh:message "maxImpedanceWheelset (1.1.1.3.7.15.2): Maximum impedance between opposite wheels of a wheelset when not TSI compilant."@en .

# maxSandingOutput: # 1.1.1.3.7.17
era-sh:TrainDetectionSystemShape sh:property era-sh:maxSandingOutput .
era-sh:maxSandingOutput
	a sh:PropertyShape ;
	rdfs:comment "Maximum amount of sand whithin 30s given in grams accepted on the track." ;
	era:rinfIndex "1.1.1.3.7.17" ;
	sh:path era:maxSandingOutput ;
	sh:minCount 0 ; # TODO: Not yet applicable
	sh:nodeKind sh:IRI ;
#	sh:class skos:Concept ; #TODO: Check error	
	skos:inScheme era-mas:MaxAmountSandings ;
	sh:severity sh:Violation ;
	sh:message "maxSandingOutput (1.1.1.3.7.17): Maximum amount of sand whithin 30s given in grams accepted on the track."@en .

# requiredSandingOverride: # 1.1.1.3.7.18
era-sh:TrainDetectionSystemShape sh:property era-sh:requiredSandingOverride .
era-sh:requiredSandingOverride
	a sh:PropertyShape ;
	rdfs:comment "Indication of whether sanding override by driver required." ;
	era:rinfIndex "1.1.1.3.7.18" ;
	sh:path era:requiredSandingOverride ;
	sh:minCount 0 ; # TODO: Not yet applicable
	sh:datatype xsd:boolean ;
	sh:severity sh:Violation ;
	sh:message "requiredSandingOverride (1.1.1.3.7.18): Indication of whether sanding override by driver required."@en .

# tsiCompliantSandCharacteristics: # 1.1.1.3.7.19
era-sh:TrainDetectionSystemShape sh:property era-sh:tsiCompliantSandCharacteristics .
era-sh:tsiCompliantSandCharacteristics
	a sh:PropertyShape ;
	rdfs:comment "Indication of whether the rules are TSI compliant on sand characteristics." ;
	era:rinfIndex "1.1.1.3.7.19" ;
	sh:path era:tsiCompliantSandCharacteristics ;
	sh:minCount 0 ; # TODO: Not yet applicable
	sh:nodeKind sh:IRI ;
#	sh:class skos:Concept ; #TODO: Check error
	skos:inScheme era-tsi:TSICompliances ;
	sh:severity sh:Violation ;
	sh:message "tsiCompliantSandCharacteristics (1.1.1.3.7.19): Indication of whether the rules are TSI compliant on sand characteristics."@en .

# flangeLubeRules: # 1.1.1.3.7.20
era-sh:TrainDetectionSystemShape sh:property era-sh:flangeLubeRules .
era-sh:flangeLubeRules
	a sh:PropertyShape ;
	rdfs:comment "Indication whether rules for activation or deactivation of flange lubrication exist." ;
	era:rinfIndex "1.1.1.3.7.20" ;
	sh:path era:flangeLubeRules ;
	sh:minCount 0 ; # TODO: Not yet applicable
	sh:datatype xsd:boolean ;
	sh:severity sh:Violation ;
	sh:message "flangeLubeRules (1.1.1.3.7.20): Indication of whether the rules are TSI compliant for flange lubrication."@en .

# tsiCompliantCompositeBrakeBlocks: # 1.1.1.3.7.21
era-sh:TrainDetectionSystemShape sh:property era-sh:tsiCompliantCompositeBrakeBlocks .
era-sh:tsiCompliantCompositeBrakeBlocks
	a sh:PropertyShape ;
	rdfs:comment "Indication of whether the rules are TSI compliant on composite brake blocks." ;
	era:rinfIndex "1.1.1.3.7.21" ;
	sh:path era:tsiCompliantCompositeBrakeBlocks ;
	sh:minCount 0 ; # TODO: Not yet applicable
	sh:nodeKind sh:IRI ;
#	sh:class skos:Concept ; #TODO: Check error
	skos:inScheme era-tsi:TSICompliances ;
	sh:severity sh:Violation ;
	sh:message "tsiCompliantCompositeBrakeBlocks (1.1.1.3.7.21): Indication of whether the rules are TSI compliant for composite brake blocks."@en .

# tsiCompliantShuntDevices: # 1.1.1.3.7.22
era-sh:TrainDetectionSystemShape sh:property era-sh:tsiCompliantShuntDevices .
era-sh:tsiCompliantShuntDevices
	a sh:PropertyShape ;
	rdfs:comment "Indication of whether the rules are TSI compliant on shunt assisting devices." ;
	era:rinfIndex "1.1.1.3.7.22" ;
	sh:path era:tsiCompliantShuntDevices ;
	sh:minCount 0 ; # TODO: Not yet applicable
	sh:nodeKind sh:IRI ;
#	sh:class skos:Concept ; #TODO: Check error
	skos:inScheme era-tsi:TSICompliances ;
	sh:severity sh:Violation ;
	sh:message "tsiCompliantShuntDevices (1.1.1.3.7.22): Indication of whether the rules are TSI compliant for shunt assisting devices."@en .

# tsiCompliantRSTShuntImpedance: # 1.1.1.3.7.23
era-sh:TrainDetectionSystemShape sh:property era-sh:tsiCompliantRSTShuntImpedance .
era-sh:tsiCompliantRSTShuntImpedance
	a sh:PropertyShape ;
	rdfs:comment "Indication of whether the rules are TSI compliant on combination of RST characteristics influencing shunting impedance." ;
	era:rinfIndex "1.1.1.3.7.23" ;
	sh:path era:tsiCompliantRSTShuntImpedance ;
	sh:minCount 0 ; # TODO: Not yet applicable
	sh:nodeKind sh:IRI ;
#	sh:class skos:Concept ; #TODO: Check error
	skos:inScheme era-tsi:TSICompliances ;
	sh:severity sh:Violation ;
	sh:message "tsiCompliantRSTShuntImpedance (1.1.1.3.7.23): Indication of whether the rules are TSI compliant for combination of RST characteristics influencing shunting impedance."@en .